Removed effect tracking from derivations

Refinery/Signature.lean
@@ -17,18 +17,20 @@ def Signature.HasEff (e : ε) (f : φ) := eff f ≤ e
 theorem Signature.HasEff.mono {e e' : ε} (he : e ≤ e') {f : φ} (h : HasEff e f) : HasEff e' f
   := le_trans h he
 
-structure Signature.IsFn (f : φ) (e : ε) (A B : Ty α) where
+structure Signature.FnTy (f : φ) (A B : Ty α) where
   src : A = src f
   trg : B = trg f
+
+structure Signature.IsFn (f : φ) (e : ε) (A B : Ty α) extends FnTy f A B where
   eff : HasEff e f
 
 attribute [simp] Signature.IsFn.eff
 
 theorem Signature.IsFn.withEff {f : φ} {e e' : ε} {A B : Ty α} (h : IsFn f e A B) (he : HasEff e' f)
-  : IsFn f e' A B := ⟨h.src, h.trg, he⟩
+  : IsFn f e' A B := ⟨⟨h.src, h.trg⟩, he⟩
 
 theorem Signature.IsFn.mono {f : φ} {e e' : ε} {A B : Ty α} (h : IsFn f e A B) (he : e ≤ e')
-  : IsFn f e' A B := ⟨h.src, h.trg, h.eff.mono he⟩
+  : IsFn f e' A B := ⟨⟨h.src, h.trg⟩, h.eff.mono he⟩
 
 theorem Signature.IsFn.top {f : φ} {e : ε} {A B : Ty α} (h : IsFn f e A B) : IsFn f ⊤ A B
   := h.mono le_top
