Refinery/Term/Extrinsic/Wk.lean
@@ -7,8 +7,8 @@ namespace Term
 
 variable {φ : Type u} {α : Type v} {ε : Type w} [S : Signature φ α ε]
 
-def Deriv.wkTerm {e : ε} {Γ Δ : Ctx? α} (ρ : Γ.Wk Δ) {A : Ty α} {a : Term φ (Ty α)}
-  : (Δ ⊢[e] a : A) → Term φ (Ty α)
+def Deriv.wkTerm {Γ Δ : Ctx? α} (ρ : Γ.Wk Δ) {A : Ty α} {a : Term φ (Ty α)}
+  : (Δ ⊢ a : A) → Term φ (Ty α)
   | .bv (n := n) hv => .bv (ρ n)
   | .op (f := f) hf da => .op f (da.wkTerm ρ)
   | .let₁ (A := A) (B := B) hΓ da db =>
@@ -24,16 +24,16 @@ def Deriv.wkTerm {e : ε} {Γ Δ : Ctx? α} (ρ : Γ.Wk Δ) {A : Ty α} {a : Ter
     .case (da.wkTerm (hΓ.rightWk ρ)) A B (db.wkTerm ((hΓ.leftWk ρ).scons _))
           (dc.wkTerm ((hΓ.leftWk ρ).scons _))
   | .abort (A := A) da => .abort A (da.wkTerm ρ)
-  | .iter (A := A) (B := B) hΓ _ _ _ da db =>
+  | .iter (A := A) (B := B) hΓ _ _ da db =>
     .iter (da.wkTerm (hΓ.rightWk ρ)) A B (db.wkTerm ((hΓ.leftWk ρ).scons _))
 
 @[simp]
-theorem Deriv.wkTerm_eq {e : ε} {Γ Δ : Ctx? α} (ρ : Γ.Wk Δ) {A : Ty α} {a : Term φ (Ty α)}
-  (D : Δ ⊢[e] a : A) : D.wkTerm ρ = a.ren ρ
+theorem Deriv.wkTerm_eq {Γ Δ : Ctx? α} (ρ : Γ.Wk Δ) {A : Ty α} {a : Term φ (Ty α)}
+  (D : Δ ⊢ a : A) : D.wkTerm ρ = a.ren ρ
   := by induction D generalizing Γ <;> simp [wkTerm, *]
 
-def Deriv.wkD {e : ε} {Γ Δ : Ctx? α} (ρ : Γ.Wk Δ) {A : Ty α} {a : Term φ (Ty α)}
-  : (D : Δ ⊢[e] a : A) → (Γ ⊢[e] D.wkTerm ρ : A)
+def Deriv.wkD {Γ Δ : Ctx? α} (ρ : Γ.Wk Δ) {A : Ty α} {a : Term φ (Ty α)}
+  : (D : Δ ⊢ a : A) → (Γ ⊢ D.wkTerm ρ : A)
   | .bv hv => .bv (hv.wkIn ρ)
   | .op hf da => .op hf (da.wkD ρ)
   | .let₁ (A := A) (B := B) hΓ da db =>
@@ -50,12 +50,12 @@ def Deriv.wkD {e : ε} {Γ Δ : Ctx? α} (ρ : Γ.Wk Δ) {A : Ty α} {a : Term �
     .case (hΓ.wk ρ) (da.wkD (hΓ.rightWk ρ)) (db.wkD ((hΓ.leftWk ρ).scons _))
           (dc.wkD ((hΓ.leftWk ρ).scons _))
   | .abort (A := A) da => .abort (da.wkD ρ)
-  | .iter (A := A) (B := B) hΓ hei _ _ da db =>
-    .iter (hΓ.wk ρ) hei (hΓ.wkLeft_copy ρ) (hΓ.wkLeft_del ρ)
+  | .iter (A := A) (B := B) hΓ _ _ da db =>
+    .iter (hΓ.wk ρ) (hΓ.wkLeft_copy ρ) (hΓ.wkLeft_del ρ)
                         (da.wkD (hΓ.rightWk ρ)) (db.wkD ((hΓ.leftWk ρ).scons _))
 
-def Deriv.wk {e : ε} {Γ Δ : Ctx? α} (ρ : Γ.Wk Δ) {A : Ty α} {a : Term φ (Ty α)}
-  (D : Δ ⊢[e] a : A) : (Γ ⊢[e] a.ren ρ : A)
+def Deriv.wk {Γ Δ : Ctx? α} (ρ : Γ.Wk Δ) {A : Ty α} {a : Term φ (Ty α)}
+  (D : Δ ⊢ a : A) : (Γ ⊢ a.ren ρ : A)
   := (D.wkD ρ).cast_term (D.wkTerm_eq ρ)
 
 end Term
